Congruence_Closure_Explain/Congruence_Closure_Proofs.thy
@@ -1,0 +1,4 @@
+section \<open>Correctness proofs for congruence closure\<close>
+theory Congruence_Closure_Proofs
+  imports Congruence_Closure 
+begin 
