ROOT
@@ -1,8 +1,10 @@
-
-session "Congruence-Closure" = HOL +
+session "Congruence_Closure" = HOL +
   sessions
     "HOL-Library"
     Separation_Logic_Imperative_HOL
+  directories
+    Union_Find_Explain
+    Congruence_CLosure_Explain
   theories
     Explain
     Path
